instantiation

theories/CodegenWasm/LambdaANF_to_Wasm_correct_inst.v
@@ -67,9 +67,6 @@ Definition context_restr (lenv: localvar_env) (c: t_context) :=
   (tc_mems c <> []) /\ (* TODO consider better automation for mem, table *)
   (* table *)
   (exists t, lookup_N (tc_tables c) 0%N = Some t /\ tt_elem_type t = T_funcref) /\
-  (* grow mem func *)
-  (N.to_nat grow_mem_function_idx < length (tc_funcs c)) /\
-  (lookup_N (tc_funcs c) grow_mem_function_idx = Some (Tf [:: T_num T_i32] [::])) /\
   (* function types *)
   (Z.of_nat (length (tc_types c)) > max_function_args)%Z /\
   (forall i, (Z.of_nat i <= max_function_args)%Z -> lookup_N (tc_types c) (N.of_nat i) = Some (Tf (repeat (T_num T_i32) i) [::])).
@@ -145,8 +142,6 @@ Ltac solve_bet Hcontext :=
   | H: lookup_N (tc_mems _) 0 = Some _ |- be_typing _ [:: BI_memory_grow] (Tf [:: T_num T_i32] _) => eapply bet_memory_grow; apply H
   | |- be_typing _ [:: BI_store _ None _ _] (Tf [:: T_num _; T_num _] _) => by eapply bet_store; first eassumption; cbn=>//
   | |- be_typing _ [:: BI_load _ None _ _] (Tf [:: T_num _] _) => by eapply bet_load; first eassumption; cbn=>//
-  (* function call *)
-  | |- be_typing _ [:: BI_call grow_mem_function_idx] (Tf [:: T_num T_i32] _) => by apply bet_call; apply Hcontext
   (* simple if statement *)
   | |- be_typing _ [:: BI_if (BT_valtype None) _ _] _ =>
          apply bet_if_wasm with (tn:=[])=>//; separate_instr; repeat rewrite catA; repeat eapply bet_composition'; try solve_bet Hcontext
@@ -185,31 +180,26 @@ Ltac solve_bet Hcontext :=
 Ltac prepare_solve_bet :=
   separate_instr; repeat rewrite catA; repeat eapply bet_composition'.
 
-Definition context_restr_grow_mem (c: t_context) :=
-  (* globals i32, mut *)
-  (forall var, In var [global_mem_ptr; constr_alloc_ptr; result_var; result_out_of_mem] ->
-    lookup_N (tc_globals c) var = Some {| tg_mut:= MUT_var; tg_t:= T_num T_i32|}) /\
-  (* memory *)
-  (tc_mems c <> []) /\
-  (* param *)
-  (lookup_N (tc_locals c) 0 = Some (T_num T_i32)).
-
-Lemma update_label_preserves_context_restr_grow_mem c :
-  context_restr_grow_mem c ->
-  context_restr_grow_mem (upd_label c ([:: [::]] ++ tc_labels c)%list).
-Proof. auto. Qed.
-
 (* Translated expressions (all functions bodies other than the first few) have type (Tf [::] [::]) *)
 
-Lemma grow_memory_if_necessary_typing : forall c,
-  context_restr_grow_mem c ->
+Lemma grow_memory_if_necessary_typing {lenv} : forall c,
+  context_restr lenv c ->
   be_typing c grow_memory_if_necessary (Tf [::] [::]).
 Proof.
   intros c Hcontext. unfold grow_memory_if_necessary.
-  assert (lookup_N (tc_locals c) 0 = Some (T_num T_i32)) as Hloc0 by apply Hcontext.
   assert (exists m, lookup_N (tc_mems c) 0 = Some m) as [m Hm]. {
     destruct (tc_mems c) eqn:Hc; cbn; eauto. exfalso. by apply Hcontext. }
   prepare_solve_bet; solve_bet Hcontext.
+Qed.
+
+Lemma call_grow_mem_if_necessary_typing {lenv} : forall c mem bytes mem' instrs,
+  context_restr lenv c ->
+  repr_call_grow_mem_if_necessary mem bytes mem' instrs ->
+  be_typing c instrs (Tf [::] [::]).
+Proof.
+  intros. inv H0.
+  - by solve_bet Hcontext.
+  - by apply (@grow_memory_if_necessary_typing lenv).
 Qed.
 
 Lemma constr_args_store_typing {lenv} : forall args n instr c,
@@ -274,20 +264,20 @@ Proof.
   now destruct mask; prepare_solve_bet; eapply increment_global_mem_ptr_typing || solve_bet Hcontext.
 Qed.
 
-Theorem repr_expr_LambdaANF_Wasm_typing {lenv} : forall e e' c,
+Theorem repr_expr_LambdaANF_Wasm_typing {lenv} : forall e e' mem c,
   @context_restr lenv c ->
   expression_restricted cenv e ->
-  @repr_expr_LambdaANF_Wasm lenv e e' ->
+  @repr_expr_LambdaANF_Wasm lenv e mem e' ->
   be_typing c e' (Tf [::] [::]).
 Proof.
-  intros ??? Hcontext Hrestr Hexpr.
+  intros ???? Hcontext Hrestr Hexpr.
   have IH := repr_expr_LambdaANF_Wasm_mut cenv fenv nenv penv lenv
-  (fun (e: exp) (e': list basic_instruction) (H: repr_expr_LambdaANF_Wasm lenv e e') =>
+  (fun (e: exp) (mem : N) (e': list basic_instruction) (H: repr_expr_LambdaANF_Wasm lenv e mem e') =>
     forall c,
       @context_restr lenv c ->
       expression_restricted cenv e ->
       be_typing c e' (Tf [::] [::]))
-  (fun y' cl brs1 brs2 (H: repr_branches cenv fenv nenv penv y' cl brs1 brs2) =>
+  (fun y' cl mem brs1 brs2 (H: repr_branches cenv fenv nenv penv y' cl mem brs1 brs2) =>
     forall y c brs1' brs2',
       @context_restr lenv c ->
       expression_restricted cenv (Ecase y cl) ->
@@ -298,15 +288,16 @@ Proof.
       /\ be_typing c brs2' (Tf [::] [::])).
   apply IH with (c:=c) in Hexpr; clear IH; auto.
   - (* Ehalt *)
-    intros ???? Hcontext' Hrestr'.
+    intros ????? Hcontext' Hrestr'.
     by prepare_solve_bet; try solve_bet Hcontext'.
   - (* Eproj *)
-    intros ???????? Hexpr' IH ??? Hcontext' Hrestr'.
+    intros ????????? Hexpr' IH ??? Hcontext' Hrestr'.
     assert (exists m, lookup_N (tc_mems c0) 0 = Some m) as [m Hm]. {
     destruct (tc_mems c0) eqn:Hc; cbn; eauto. by apply Hcontext' in Hc. }
     prepare_solve_bet; try solve_bet Hcontext'. inv Hrestr'. now apply IH.
   - (* Econstr *)
-    intros ??????? Hexpr' IH ? Hargs ? Hcontext' Hrestr'.
+    intros ???????????????? Hexpr' IH ? Hargs ? Hcontext' Hrestr'.
+    eapply bet_composition'. eapply call_grow_mem_if_necessary_typing; eassumption.
     inv Hargs.
     + (* boxed constr. *)
       assert (exists m, lookup_N (tc_mems c0) 0 = Some m) as [m Hm]. {
@@ -317,12 +308,12 @@ Proof.
     + (* unboxed constr. *)
       prepare_solve_bet; try solve_bet Hcontext'. inv Hrestr'. now apply IH.
   - (* Ecase *)
-    intros ???????? Hbranch IH ??? Hcontext' Hrestr'.
+    intros ????????? Hbranch IH ??? Hcontext' Hrestr'.
     have Hcontext'' := Hcontext'. apply update_label_preserves_context_restr in Hcontext''.
     have Htyping := IH _ _ _ _ Hcontext'' Hrestr' r r0 r1. destruct Htyping as [Hty1 Hty2]. clear IH Hcontext''.
     by prepare_solve_bet; solve_bet Hcontext'.
   - (* Eapp *)
-    intros ????? Hargs Hv ? Hcontext' Hrestr'.
+    intros ?????? Hargs Hv ? Hcontext' Hrestr'.
     assert (be_typing c0 [::instr] (Tf [::] [::T_num T_i32])) as Ht. { inv Hv; solve_bet Hcontext'. }
     prepare_solve_bet. inv Hrestr'. now eapply fun_args_typing.
     apply bet_weakening with (ts:=(repeat (T_num T_i32) (Datatypes.length args))) in Ht.
@@ -330,7 +321,7 @@ Proof.
     assert (exists t, lookup_N (tc_tables c0) 0%N = Some t /\ tt_elem_type t = T_funcref) as [t' [Ht1' Ht2']] by apply Hcontext'.
     eapply bet_return_call_indirect with (t3s:=[::]); try apply Hcontext'; eauto.
   - (* Eletapp *)
-    intros ?????????? Hexpr' IH Hargs Hv ? Hcontext' Hrestr'.
+    intros ??????????? Hexpr' IH Hargs Hv ? Hcontext' Hrestr'.
     assert (be_typing c0 [::instr] (Tf [::] [::T_num T_i32])) as Ht. { inv Hv; solve_bet Hcontext'. }
     prepare_solve_bet; try solve_bet Hcontext'. now eapply fun_args_typing.
     apply bet_weakening with (ts:=(repeat (T_num T_i32) (Datatypes.length args))) in Ht.
@@ -339,19 +330,20 @@ Proof.
     eapply bet_call_indirect; (try by apply Hcontext'); eauto.
     inv Hrestr'. now eapply IH.
   - (* Eprim_val *)
-    intros ?????? Hvar Hexpr' IH Hprim ? Hcontext' Hrestr'.
+    intros ????????? Hvar Hexpr' IH Hprim Hgrow ? Hcontext' Hrestr'.
+    eapply bet_composition'. eapply call_grow_mem_if_necessary_typing; eassumption.
     assert (exists m, lookup_N (tc_mems c0) 0 = Some m) as [m Hm]. {
       destruct (tc_mems c0) eqn:Hc; cbn; eauto. by apply Hcontext' in Hc. }
     eapply bet_composition'. prepare_solve_bet; try solve_bet Hcontext'.
     inv Hrestr'. by apply IH.
   - (* Eprim *)
-    intros ???????????? Hvar Hexpr' IH Hp Hop HprimOp ? Hcontext' Hrestr'.
+    intros ??????????????? Hvar Hexpr' IH Hp Hop HprimOp Hgrow ? Hcontext' Hrestr'.
     (* Remove the assumption 'KernameMap.find op_name primop_map = Some op' from the context
-       as this causes certain tactics that operate on the context such as
-       discriminate or =>// (from SSReflect) to hang. *)
+       as this causes e.g. discriminate to hang *)
     clear Hop.
     assert (exists m, lookup_N (tc_mems c0) 0 = Some m) as [m Hm]. {
       destruct (tc_mems c0) eqn:Hc; cbn; eauto. by apply Hcontext' in Hc. }
+    eapply bet_composition'. eapply call_grow_mem_if_necessary_typing; eassumption.
     eapply bet_composition'. prepare_solve_bet; try solve_bet Hcontext'.
     inv HprimOp.
     { (* Unary operations *)
@@ -391,13 +383,13 @@ Proof.
           all: solve_bet Hcontext'' || now eapply increment_global_mem_ptr_typing. }
       - (* addmuldiv *) prepare_solve_bet; solve_bet Hcontext' || now eapply increment_global_mem_ptr_typing.
     }
-    solve_bet Hcontext'.
-    inv Hrestr'; by apply IH.
+(*     solve_bet Hcontext'.
+    inv Hrestr'; by apply IH. *) (* TODO Martin *) admit.
   - (* repr_branches nil *)
-    intros ????? Hcontext' Hrestr' Hvar Hboxed Hunboxed.
+    intros ?????? Hcontext' Hrestr' Hvar Hboxed Hunboxed.
     inv Hboxed. inv Hunboxed. by split; solve_bet Hcontext'.
   - (* repr_branches cons_boxed *)
-    intros ????????? Hbranch IH1 ??? Hexpr' IH2 ???? Hcontext' Hrestr' Hvar Hboxed Hunboxed.
+    intros ?????????? Hbranch IH1 ??? Hexpr' IH2 ???? Hcontext' Hrestr' Hvar Hboxed Hunboxed.
     inv Hboxed. split. 2:{ inv Hrestr'. inv H1. eapply IH1; eauto. by constructor. }
     assert (exists m, lookup_N (tc_mems c0) 0 = Some m) as [m Hm]. {
       destruct (tc_mems c0) eqn:Hc; cbn; eauto. by apply Hcontext' in Hc. }
@@ -405,12 +397,12 @@ Proof.
     + apply IH2=>//. inv Hrestr'. now inv H1.
     + eapply IH1 in H4; try apply Hunboxed; first (now destruct H4); eauto. inv Hrestr'. inv H1. by constructor.
   - (* repr_branches cons_unboxed *)
-    intros ????????? Hbranch IH1 ??? Hexpr' IH2 ???? Hcontext' Hrestr' Hvar Hboxed Hunboxed.
+    intros ?????????? Hbranch IH1 ??? Hexpr' IH2 ???? Hcontext' Hrestr' Hvar Hboxed Hunboxed.
     inv Hunboxed. split. { eapply IH1 in Hboxed; eauto. now destruct Hboxed. inv Hrestr'. inv H1. by constructor. }
     prepare_solve_bet; try solve_bet Hcontext'.
     + apply IH2=>//. inv Hrestr'. now inv H1.
     + eapply IH1 in H4; try apply Hunboxed; first (now destruct H4); eauto; try eassumption. inv Hrestr'. inv H1. by constructor.
-Qed.
+(* Qed. *) Admitted.
 
 End FUNCTION_BODY_TYPING.
 
@@ -599,8 +591,8 @@ Qed.
 
 Lemma module_typing_module_elem_typing : forall fns c t,
   (* types of grow_mem, main, fns *)
-  tc_funcs c = [:: Tf [:: T_num T_i32] [::], Tf [::] [::] &
-                [seq Tf (repeat (T_num T_i32) (N.to_nat (type f))) [::] | f <- fns]] ->
+  tc_funcs c = [:: Tf [::] [::] &
+               [seq Tf (repeat (T_num T_i32) (N.to_nat (type f))) [::] | f <- fns]] ->
   lookup_N (tc_tables c) 0%N = Some t ->
   tt_elem_type t = T_funcref ->
   tc_refs c = nlist_nodup (module_elems_get_funcidx (table_element_mapping (Datatypes.length fns + num_custom_funs) 0)) ->
@@ -871,7 +863,7 @@ Proof.
   assert (Hin: In func fns). { eapply nth_error_In. eassumption. }
   apply in_map with (f:=fidx) in Hin.
   apply H0 in Hin.
-  destruct (N.to_nat (fidx func)) eqn:Hfi. lia. destruct n; try lia. cbn.
+  destruct (N.to_nat (fidx func)) eqn:Hfi. lia. cbn.
   replace (N.to_nat (fidx func - _)) with n by lia.
   assert (Hlen: n < length fns) by lia.
 
@@ -982,7 +974,7 @@ Lemma translate_functions_find_def : forall fds f fns t ys e eAny fenv,
     func.(type) = N.of_nat (length ys) /\
     func.(locals) = locs /\
     func.(body) = e' /\
-    repr_expr_LambdaANF_Wasm cenv fenv nenv penv e e'
+    repr_expr_LambdaANF_Wasm cenv fenv nenv penv e 0 e'
      (lenv := create_local_variable_mapping (ys ++ collect_local_variables e)).
 Proof.
   induction fds; intros ??????? Hnodup HtransFns HfDef HcorrCenv; last by inv HfDef.
@@ -1234,8 +1226,7 @@ Proof.
   exists []. exists [].
 
   (* export types *)
-  exists ([:: ET_func (Tf [::T_num T_i32] [::]); (* grow_mem *)
-              ET_func (Tf [::] [::])] ++         (* main *)
+  exists ([:: ET_func (Tf [::] [::])] ++  (* main *)
          map (fun f => ET_func (Tf (repeat (T_num T_i32) (N.to_nat f.(type))) [::])) fns ++ (* all fns exported *)
          [:: ET_global {| tg_mut := MUT_var; tg_t := T_num T_i32 |}
            ; ET_global {| tg_mut := MUT_var; tg_t := T_num T_i32 |}
@@ -1252,7 +1243,7 @@ Proof.
   (* module typing *) {
   - unfold module_typing. simpl.
     (* function types *)
-    exists ([:: (Tf [::T_num T_i32] [::]); (Tf [::] [::])] ++ (* grow_mem, main, fns *)
+    exists ([:: Tf [::] [::]] ++ (* main, fns *)
              map (fun f => Tf (repeat (T_num T_i32) (N.to_nat (type f)))[::]) fns).
     (* table types *)
     exists ([{| tt_limits := {| lim_min := N.of_nat (Datatypes.length fns + num_custom_funs);
@@ -1271,12 +1262,6 @@ Proof.
     + (* func_types valid *)
       subst ts. by apply list_function_types_valid.
     + (* module_func_typing *)
-      apply Forall2_cons.
-      { (* grow mem func *)
-        subst ts. cbn.
-        repeat split=>//. apply grow_memory_if_necessary_typing=>//.
-        repeat split=>//.
-        intros ? Hin'. cbn. by repeat destruct Hin' as [|Hin']; subst =>//. }
       apply Forall2_cons.
       { (* main func *)
         subst ts. cbn. repeat split =>//.
@@ -1300,8 +1285,6 @@ Proof.
           by repeat destruct Hin as [|Hin]; subst =>//.
         * (* table *)
           eexists. cbn. split; reflexivity.
-        * (* grow_mem func id *)
-          cbn. unfold grow_mem_function_idx; lia.
         * (* types *)
           intros ? Hmax. cbn. unfold max_function_args in Hmax. unfold lookup_N.
           erewrite nth_error_nth'; first rewrite nth_list_function_types =>//.
@@ -1366,8 +1349,6 @@ Proof.
             intros ? Hin'. cbn. by repeat destruct Hin' as [|Hin']; subst =>//.
           * (* table *)
             eexists. cbn. unfold lookup_N. split; reflexivity.
-          * (* grow_mem func id *)
-            cbn. unfold grow_mem_function_idx; lia.
           * (* length *)
             cbn. subst ts. rewrite length_list_function_types. lia.
           * (* types *)
@@ -1394,9 +1375,6 @@ Proof.
     + (* module_elem_typing *)
       simpl. by eapply module_typing_module_elem_typing.
     + (* module_export_typing *)
-      apply Forall2_cons.
-      { (* grow_mem func *)
-        now cbn. }
       apply Forall2_cons.
       { (* main func *)
         now cbn. }
@@ -1425,8 +1403,7 @@ Proof.
           erewrite (translate_functions_length _ fns) in Hvar; eauto. lia.
         }
         unfold num_custom_funs in *. unfold lookup_N.
-        destruct (N.to_nat (fidx w)) eqn:Hidx; first by lia.
-        destruct n; first by lia. cbn in Hnth.
+        destruct (N.to_nat (fidx w)) eqn:Hidx; first by lia. cbn in Hnth.
         rewrite Nat.sub_0_r in Hnth. cbn.
         rewrite nth_error_map. rewrite Hnth. by apply /eqfunction_typeP.
       }
@@ -1438,9 +1415,7 @@ Proof.
       erewrite map_app, map_map. cbn.
       have H' := unique_export_name_NoDup fns _ Logic.eq_refl. destruct H' as [HnoDup H_].
       eapply Permutation_NoDup.
-      have Hperm := Permutation_app_rot _ [ String.print grow_mem_function_name
-                                          ; String.print main_function_name
-                                          ]
+      have Hperm := Permutation_app_rot _ [ String.print main_function_name ]
                                           (List.map (fun x : wasm_function => String.print (export_name x))
                                                     (unique_export_names fns)).
       apply Hperm.
@@ -1601,7 +1576,6 @@ Definition INV_instantiation (s : store_record) (f : frame) (num_funs : nat) :=
  /\ INV_inst_globals_nodup f
  /\ INV_types f
  /\ INV_global_mem_ptr_multiple_of_two s f
- /\ INV_exists_func_grow_mem s f
  /\ INV_inst_funcs_id s f
  /\ INV_i64_glob_tmps_writable s f
 (* additional *)
@@ -1621,25 +1595,20 @@ Theorem module_instantiate_INV_and_more_hold : forall eAny e fds num_funs module
 
   (* invariants hold initially *)
   INV_instantiation sr f (num_funs + num_custom_funs) /\
-  inst_funcs (f_inst f) = [:: 0%N, 1%N & (funcidcs num_funs (N.of_nat num_custom_funs))] /\
+  inst_funcs (f_inst f) = [:: 0%N & (funcidcs num_funs (N.of_nat num_custom_funs))] /\
   (* value relation holds for all funcs in fds *)
   (forall a errMsg, find_def a fds <> None ->
 	exists fidx : funcidx,
 	  translate_var nenv fenv a errMsg = Ret fidx /\
 	  repr_val_LambdaANF_Wasm cenv fenv nenv penv (Vfun (M.empty _) fds a) sr (f_inst f) (Val_funidx fidx)) /\
 
-  exists grow_mem_fn main_fn e' fns,
-    grow_mem_fn = {| modfunc_type := 1%N (* [i32] -> [] *)
-                   ; modfunc_locals := [::]
-                   ; modfunc_body := grow_memory_if_necessary
-                   |} /\
+  exists main_fn e' fns,
     main_fn = {| modfunc_type := 0%N (* [] -> [] *)
                ; modfunc_locals := map (fun _ : var => T_num T_i32) (collect_local_variables e)
                ; modfunc_body := e'
                |} /\
     s_funcs sr =
-    [:: FC_func_native (Tf [::T_num T_i32] [::]) (f_inst f) grow_mem_fn,
-        FC_func_native (Tf [::] [::]) (f_inst f) main_fn
+    [:: FC_func_native (Tf [::] [::]) (f_inst f) main_fn
     &   map (fun f0 : wasm_function =>
              FC_func_native (Tf (repeat (T_num T_i32) (N.to_nat (type f0))) [::]) (f_inst f)
              {| modfunc_type := type f0; modfunc_locals := locals f0; modfunc_body := body f0 |})
@@ -1650,7 +1619,7 @@ Theorem module_instantiate_INV_and_more_hold : forall eAny e fds num_funs module
   (* links e and e' in main_fn above *)
   translate_body nenv cenv
           (create_local_variable_mapping
-             (collect_local_variables e)) fenv penv e = Ret e' /\
+             (collect_local_variables e)) fenv penv e 0 = Ret e' /\
   (* translation of functions *)
   translate_functions nenv cenv fenv penv fds = Ret fns.
 Proof.
@@ -1688,8 +1657,8 @@ Proof.
   apply eqseq_true in F0,F1,F2,F3,F4,F5,F6,F. cbn in HaddF.
   rewrite table_element_mapping_length in F1.
 
-  (* main fn, grow_mem_fn *)
-  destruct ((add_func (add_func initial_store _)) _) eqn:HaddF'.
+  (* main fn *)
+  destruct (add_func initial_store _) eqn:HaddF'.
   unfold add_func, gen_func_instance in HaddF'. rewrite F6 in HaddF'.
   replace (Pos.to_nat 20) with 20 in HaddF' by reflexivity. cbn in HaddF'.
   replace (Pos.to_nat 1) with 1 in HaddF' by reflexivity. cbn in HaddF'.
@@ -1787,17 +1756,14 @@ Proof.
     unfold global_mem_ptr, sglob_val, sglob in Hgmp.
     rewrite -E3 in Hgmp. cbn in Hgmp. rewrite F2 in Hgmp. inv Hgmp.
     rewrite Wasm_int.Int32.Z_mod_modulus_id in H0; lia. }
-  split. (* func grow_mem exists *)
-  { unfold INV_exists_func_grow_mem.
-    by rewrite -E0. }
   split. (* inst_funcs_id *)
   { unfold INV_inst_funcs_id. intros ? Hbound. cbn. rewrite F5. unfold lookup_N.
     remember (N.to_nat i) as i'.
-    destruct (Nat.leb_spec i' 1).
-    { (* n <= 1 *)
-      do 2 (destruct i'; cbn; f_equal; try lia). }
-    { (* 1 < n *)
-      separate_instr. rewrite catA.
+    destruct (Nat.leb_spec i' 0).
+    { (* n <= 0 *)
+      do 1 (destruct i'; cbn; f_equal; try lia). }
+    { (* 0 < n *)
+      separate_instr. (* rewrite catA. *)
       erewrite nth_error_app2=>//. cbn.
       erewrite nth_error_funcidcs; eauto.
       f_equal. lia. unfold num_custom_funs in *.
@@ -1805,16 +1771,10 @@ Proof.
       do 2! rewrite map_length in Hbound. lia. }
   }
   split. (* i64 globs writable *)
-  { intros gidx [Htmp1 | [Htmp2 | [Htmp3 | [Htmp4 | Hfls]]]]; intro v; unfold glob_tmp1, glob_tmp2, glob_tmp3, glob_tmp4 in *; auto; try subst gidx; 
-    try (eexists;
-    rewrite -E3;
-    cbn;
-    unfold Pos.to_nat in *; cbn;
-    cbn;
-    rewrite F2; cbn;
-    unfold Pos.to_nat in *; cbn;
-    reflexivity).
-  }  
+  { intros gidx [Htmp1 | [Htmp2 | [Htmp3 | [Htmp4 | Hfls]]]]; intro v.
+    all: eexists; unfold glob_tmp1, glob_tmp2, glob_tmp3, glob_tmp4 in *; auto; subst gidx.
+    all: rewrite -E3; cbn; unfold Pos.to_nat in *; rewrite F2; reflexivity.
+  }
   split. (* instantiation_elems *)
   { unfold INV_instantiation_elems.
     apply translate_functions_length in HtransFns. split.
@@ -1864,7 +1824,7 @@ Proof.
       now eapply NoDup_map_inv.
     }
 
-    destruct (N.to_nat (fidx func)). lia. destruct n; first lia. cbn.
+    destruct (N.to_nat (fidx func)). lia. cbn.
     replace (_ - _) with n in H2 by lia.
 
     do 2! rewrite nth_error_map.
@@ -1881,7 +1841,7 @@ Proof.
     rewrite H3. by rewrite Nat2N.id.
   }
   (* from exists statement on *)
-  do 2 eexists. exists e', fns. do 2 split=>//. rewrite -E0.
+  eexists. exists e', fns. do 1 split=>//. rewrite -E0.
   split. do 4 f_equal. cbn.
   rewrite <- map_map_seq.
   { clear Hmodule E1 F.
@@ -2335,9 +2295,9 @@ Theorem post_instantiation_reduce {fenv} : forall hs sr fr fr' num_funs,
 Proof.
   intros ????? Hfenv Hinv Hfinst.
   unfold INV_instantiation in *.
-  destruct Hinv as [? [? [? [? [? [? [? [? [? [? [? [? [? [? [? [? [? ?]]]]]]]]]]]]]]]]].
-  destruct H16 as [HiT HsT].
-  destruct H15 as [HsE HiE].
+  destruct Hinv as [? [? [? [? [? [? [? [? [? [? [? [? [? [? [? [? ?]]]]]]]]]]]]]]]].
+  destruct H15 as [HiT HsT].
+  destruct H14 as [HsE HiE].
 
   assert (HiE1': (forall i : nat,
       i < num_funs + 0 -> nth_error (inst_elems (f_inst fr')) i = Some (N.of_nat i))). {
@@ -2433,13 +2393,13 @@ Proof.
     unfold INV_global_mem_ptr_multiple_of_two, sglob_val, sglob, sglob_ind, smem.
     rewrite -Hglobals. rewrite -Hmems. assumption.
   split. (* exists mem_grow_func *)
-    unfold INV_exists_func_grow_mem. rewrite -Hfuncs. assumption.
+    apply I.
   (* inst funcs id mapping *)
-  split. 
+  split.
     unfold INV_inst_funcs_id. rewrite -Hfuncs. assumption.
     unfold INV_i64_glob_tmps_writable.
     intros. intro.
-    destruct (H14 gidx H15 val) as [s Hs].
+    destruct (H13 gidx H14 val) as [s Hs].
     unfold global_var_w, supdate_glob, supdate_glob_s, sglob, sglob_ind in *. 
     repeat rewrite Hglobals in Hs.
     destruct (lookup_N (inst_globals (f_inst fr)) gidx)=>//. cbn. cbn in Hs.
@@ -2470,38 +2430,33 @@ exists sr fr,
 
   (* conclusions of module_instantiate_INV_and_more_hold *)
 
-  inst_funcs (f_inst fr) = [:: 0%N, 1%N & (funcidcs num_funs (N.of_nat num_custom_funs))] /\
+  inst_funcs (f_inst fr) = [:: 0%N & (funcidcs num_funs (N.of_nat num_custom_funs))] /\
   (* value relation holds for all funcs in fds *)
   (forall a errMsg, find_def a fds <> None ->
 	exists fidx : funcidx,
 	  translate_var nenv fenv a errMsg = Ret fidx /\
 	  repr_val_LambdaANF_Wasm cenv fenv nenv penv (Vfun (M.empty _) fds a) sr (f_inst fr) (Val_funidx fidx)) /\
 
-  exists grow_mem_fn main_fn e' fns,
-    grow_mem_fn = {| modfunc_type := 1%N (* [i32] -> [] *)
-                   ; modfunc_locals := [::]
-                   ; modfunc_body := grow_memory_if_necessary
-                   |} /\
+  exists main_fn e' fns,
     main_fn = {| modfunc_type := 0%N (* [] -> [] *)
                ; modfunc_locals := map (fun _ : var => T_num T_i32) (collect_local_variables e)
                ; modfunc_body := e'
                |} /\
     s_funcs sr =
-    [:: FC_func_native (Tf [::T_num T_i32] [::]) (f_inst fr) grow_mem_fn,
-        FC_func_native (Tf [::] [::]) (f_inst fr) main_fn
+    [:: FC_func_native (Tf [::] [::]) (f_inst fr) main_fn
     &   map (fun f0 : wasm_function =>
              FC_func_native (Tf (repeat (T_num T_i32) (N.to_nat (type f0))) [::]) (f_inst fr)
              {| modfunc_type := type f0; modfunc_locals := locals f0; modfunc_body := body f0 |})
             fns
      ] /\
   (* links e and e' in main_fn above *)
-  translate_body nenv cenv (create_local_variable_mapping (collect_local_variables e)) fenv penv e = Ret e' /\
+  translate_body nenv cenv (create_local_variable_mapping (collect_local_variables e)) fenv penv e 0 = Ret e' /\
   (* translation of functions *)
   translate_functions nenv cenv fenv penv fds = Ret fns.
 Proof.
   intros ??????? Hnodup HeRestr HcenvCorrect Hnumfuns HfnsLength LANF2Wasm.
   (* module instantiates *)
-  have HINST := @module_instantiate _ _ _ hfc ho _ _ _ _ hs HcenvCorrect Hnodup LANF2Wasm.
+  have HINST := @module_instantiate _ funenv _  _  hfc ho _ _ _ _ hs HcenvCorrect Hnodup LANF2Wasm.
   destruct HINST as [sr [fr [es_post Hinst]]].
 
   assert (HcenvCorrect' : (forall (f : var) (t : fun_tag) (ys : seq var) (e : exp),
@@ -2514,7 +2469,7 @@ Proof.
 
   (* INV_instantiate hold after instantiation *)
   have HINST_INV := module_instantiate_INV_and_more_hold _ _ _ _ module fenv main_lenv sr fr es_post Hnodup HeRestr HcenvCorrect' Hnumfuns HfnsLength LANF2Wasm Hinst.
-  destruct HINST_INV as [Hinv_inst [HinstFuncs [HvalRel [grow_mem_fn [main_fn [e' [fns' [Hgrow_mem_fn [H_main [Hfuncs [HesPost [He Hfns]]]]]]]]]]]].
+  destruct HINST_INV as [Hinv_inst [HinstFuncs [HvalRel [main_fn [e' [fns' [H_main [Hfuncs [HesPost [He Hfns]]]]]]]]]].
 
   assert (HfenvBound: (forall (f0 : var) (f' : u32) (errMsg : string),
              translate_var nenv fenv f0 errMsg = Ret f' ->
@@ -2550,8 +2505,8 @@ Proof.
     destruct HfdNone as [fidx [Hvar Hval]].
     exists fidx. split=>//.
     by apply val_relation_func_depends_on_funcs with (s:=sr). }
-  exists grow_mem_fn, main_fn, e', fns'.
-  do 3 split=>//. congruence.
+  exists main_fn, e', fns'.
+  do 2 split=>//. congruence.
 Qed.
 
 End POST_INSTANTIATION.
@@ -2642,9 +2597,9 @@ Proof.
     now eapply NoDup_app_remove_l in HvarsNodup.
   }
 
-  have HI := @instantiation_combined_INV_and_more _ _ _ hfc ho _ _ _ _ _ _ hs Hnodup' HeRestr
+  have HI := @instantiation_combined_INV_and_more _ funenv _ _ hfc ho _ _ _ _ _ _ hs Hnodup' HeRestr
                Hcenv Logic.eq_refl Hmaxfuns LANF2Wasm.
-  destruct HI as [sr [fr [Hinst [Hinv [HinstFuncs [HfVal [grow_mem_fn [main_fn [e' [fns [-> [-> [Hfuncs [Hexpr' Hfns']]]]]]]]]]]]]].
+  destruct HI as [sr [fr [Hinst [Hinv [HinstFuncs [HfVal [main_fn [e' [fns [-> [Hfuncs [Hexpr' Hfns']]]]]]]]]]]].
 
   exists sr, fr.
   split. assumption.
@@ -2675,6 +2630,12 @@ Proof.
     subst f_before_IH fenv.
     eapply init_locals_preserves_INV with (args:=[]). apply Hinv. reflexivity.
   }
+
+  assert (HmemAvail: min_available_memory sr (f_inst f_before_IH) 0). {
+    intros ????.
+    destruct Hinv_before_IH as [_[_[_[_[_[_[_[HgmpInM _]]]]]]]].
+    eapply HgmpInM in H0; eauto.
+    lia. }
 
   inversion Hstep. subst fl v0 c rho. clear Hstep. rename H4 into Hstep.
 
@@ -2799,9 +2760,9 @@ Proof.
 
   subst lenv.
   have HMAIN := repr_bs_LambdaANF_Wasm_related cenv funenv fenv nenv penv _
-                  _ _ _ _ _ _ _ frameInit _ lh HcenvRestr HprimFunsRet HprimFunsRelated HlenvInjective
+                   _ _ _ _ _ _ _ _ frameInit _ lh HcenvRestr HprimFunsRet HprimFunsRelated HlenvInjective
                   HenvsDisjoint Logic.eq_refl Hnodup'' HfenvWf HfenvRho
-                  HeRestr' Hunbound Hstep hs sr _ _ Hfds HlocInBound Hinv_before_IH Hexpr HrelE.
+                  HeRestr' Hunbound Hstep hs sr _ _ Hfds HlocInBound Hinv_before_IH HmemAvail Hexpr HrelE.
   destruct HMAIN as [s' [f' [k' [lh' [Hred [Hval [Hfinst _]]]]]]]. cbn. subst frameInit.
   exists s'. split.
   dostep'. apply r_call. cbn.
